\begin{figure}[!htbp]
    \centering
    \begin{align*}
        e &::=\; x \;|\; v \;|\; (e\; e\;\ldots) \;|\; (\textbf{if}\; e\; e\; e) \;|\; (p1\; e) \;|\; (p2\; e\; e) \\
          &\;\hspace*{1.3em}|\; (\textbf{set!}\; x\; e) \;|\; (\textbf{begin}\; e\; e\;\ldots) \;|\; (\textbf{lambda}\; (x_{\_}\;\ldots)\; e) \\
          &\;\hspace*{1.3em}|\; (\textbf{let-values}\; (((x_{\_})\; e)\;\ldots)\; e) \;|\; (\textbf{raises}\; e)\\
        v &::=\; n \;|\; b \;|\; c \;|\; (\textbf{void})\\
        c &::=\; (\textbf{closure}\; x\;\ldots\; e\; \Sigma)\\
        n &::=\; \textit{number}\\
        b &::=\; \textbf{true} \;|\; \textbf{false}\\
        x &::=\; \textit{variable-not-otherwise-mentioned}\\
        p1 &::=\; \textbf{add1}\\
        p2 &::=\; + \;|\; * \;|\; <\\
        o &::=\; p1 \;|\; p2\\
        E &::=\; [] \;|\; (v\;\ldots\; E\; e\;\ldots) \;|\; (o\; v\;\ldots\; E\; e\;\ldots) \;|\; (\textbf{if}\; E\; e\; e)\\
          &\;\hspace*{1.3em}|\; (\textbf{begin}\; v\;\ldots\; E\; e\;\ldots) \;|\; (\textbf{set!}\; x\; E) \\
          &\;\hspace*{1.3em}|\; (\textbf{let-values}\; (((x)\; v)\;\ldots\; ((x)\; E)\; ((x)\; e)\;\ldots)\; e)\\
        \Sigma &::=\; ((x\; \textit{any})\;\ldots)\\
        \sigma &::=\; ((x\; \textit{any})\;\ldots)
    \end{align*}

    \vspace{-1em}

    \caption{Linklet Kernel Language Grammar}
\end{figure}
